More tentative work in src/Alloc.v

src/Alloc.v
@@ -1,9 +1,16 @@
 Require Import
   Fiat.ADT
+  Fiat.Computation.IfDec
   Fiat.ADTNotation
   Hask.Data.Monoid
   Coq.Sets.Ensembles
-  Coq.Arith.Arith.
+  Coq.Lists.List
+  Coq.Arith.Arith
+  Coq.omega.Omega.
+
+Require Import
+  Fiat.ADTRefinement
+  Fiat.ADTRefinement.BuildADTRefinements.
 
 Open Scope string_scope.
 Open Scope bool_scope.
@@ -20,16 +27,28 @@ Definition Len := nat.
 
 Definition no_meaning {a : Type} : Comp a := Empty_set a.
 
-Definition HeapSpec `{Monoid a} := Def ADT {
+Definition guard (P : Prop) :=
+  { _ : () | P }.
+
+Section Alloc.
+
+Context `{Monoid a}.
+
+(** This specification for heaps is "ideal" in the sense that it assumes a
+    machine with unlimited memory and clients who use the heap appropriately;
+    thus it only specifies the meaning of allocation when memory is always
+    available and used properly. *)
+Definition IdealHeap := Def ADT {
   rep := Pos -> option (Pos * Len * a),
 
   Def Constructor0 emptyS : rep := ret (fun _ => None),,
 
-  Def Method1 allocS (r : rep) (len : Len | 0 < len) : rep * Pos :=
-    addr <- { pos | forall p, pos <= p < pos + ` len -> r p = None };
+  Def Method1 allocS (r : rep) (len : Len) : rep * Pos :=
+    guard (0 < len) >>
+    addr <- { pos | forall p, pos <= p < pos + len -> r p = None };
     ret ((fun p =>
-            if (addr <=? p) && (p <? addr + ` len)
-            then Some (addr, ` len, mempty)
+            if (addr <=? p) && (p <? addr + len)
+            then Some (addr, len, mempty)
             else r p), addr),
 
   Def Method1 freeS (r : rep) (addr : Pos) : rep :=
@@ -63,6 +82,304 @@ Definition HeapSpec `{Monoid a} := Def ADT {
 
 }%ADTParsing.
 
-Require Import
-  Fiat.ADTRefinement
-  Fiat.ADTRefinement.BuildADTRefinements.
+Inductive HeapError :=
+  | ZeroLengthAllocation
+  | NoMemoryAvailable (len : Len)
+  | NoAllocationAtAddress (addr : Pos)
+  | UnallocatedMemoryAccess (addr : Pos).
+
+(** This specification include error handling. *)
+Definition RealHeap := Def ADT {
+  rep := Rep IdealHeap,         (* denotation is the same *)
+
+  Def Constructor0 emptyS : rep :=
+    callCons IdealHeap emptyS,,
+
+  Def Method1 allocS (r : rep) (len : Len) : rep * (HeapError + Pos) :=
+    If 0 <? len
+    Then
+      mpos <- { pos : option nat
+              | match pos with
+                | Some pos' =>
+                  forall p, pos' <= p < pos' + len -> r p = None
+                | None => True
+                end };
+      match mpos with
+      | Some pos' =>
+        `(r', pos) <- callMeth IdealHeap allocS r len;
+        guard (pos = pos') >>
+        ret (r', inr pos)
+      | None =>
+        ret (r, inl (NoMemoryAvailable len))
+      end
+    Else ret (r, inl ZeroLengthAllocation),
+
+  Def Method1 freeS (r : rep) (addr : Pos) : rep * (HeapError + ()) :=
+    match r addr with
+    | Some _ =>
+      r' <- callMeth IdealHeap freeS r addr;
+      ret (r', inr ())
+    | None =>
+      ret (r, inl (NoAllocationAtAddress addr))
+    end,
+
+  Def Method1 peekS (r : rep) (addr : Pos) : rep * (HeapError + a) :=
+    match r addr with
+    | Some _ =>
+      `(r', val) <- callMeth IdealHeap peekS r addr;
+      ret (r', inr val)
+    | None =>
+      ret (r, inl (UnallocatedMemoryAccess addr))
+    end,
+
+  Def Method2 pokeS (r : rep) (addr : Pos) (w : a) : rep * (HeapError + ()) :=
+    match r addr with
+    | Some _ =>
+      r' <- callMeth IdealHeap pokeS r addr w;
+      ret (r', inr ())
+    | None =>
+      ret (r, inl (UnallocatedMemoryAccess addr))
+    end
+
+}%ADTParsing.
+
+Definition empty : Comp (Rep RealHeap) :=
+  Eval simpl in callCons RealHeap emptyS.
+
+Definition alloc (r : Rep RealHeap) (len : Len) :
+  Comp (Rep RealHeap * (HeapError + Pos)) :=
+  Eval simpl in callMeth RealHeap allocS r len.
+
+Definition free (r : Rep RealHeap) (addr : Pos) :
+  Comp (Rep RealHeap * (HeapError + ())) :=
+  Eval simpl in callMeth RealHeap freeS r addr.
+
+Definition peek (r : Rep RealHeap) (addr : Pos) :
+  Comp (Rep RealHeap * (HeapError + a)) :=
+  Eval simpl in callMeth RealHeap peekS r addr.
+
+Definition poke (r : Rep RealHeap) (addr : Pos) (w : a) :
+  Comp (Rep RealHeap * (HeapError + ())) :=
+  Eval simpl in callMeth RealHeap pokeS r addr w.
+
+Record HeapR (a : Type) : Type := {
+  allocs  : list (Pos * Len);
+  values  : list (Pos * a);
+  next    : Pos;
+  heapEnd : Pos
+}.
+
+Record Valid_HeapR `(heap : HeapR a) := {
+  next_avail : forall pos len,
+    List.In (pos, len) (allocs heap) -> pos + len <= next heap;
+  next_within : next heap <= heapEnd heap;
+  values_allocated : forall pos val,
+    List.In (pos, val) (values heap) ->
+      exists pos' len',
+        List.In (pos, len') (allocs heap) /\ pos' <= pos < pos' + len'
+}.
+
+Program Definition allocR (len : Len) (heap : HeapR a) :
+  HeapR a * (HeapError + Pos) :=
+  match 0 <? len with
+  | true =>
+    match next heap + len <=? heapEnd heap with
+    | true =>
+      ({| allocs  := (next heap, len) :: allocs heap
+        ; values  := values heap
+        ; next    := next heap + len
+        ; heapEnd := heapEnd heap
+        |}, inr (next heap))
+    | false => (heap, inl (NoMemoryAvailable len))
+    end
+  | false => (heap, inl ZeroLengthAllocation)
+  end.
+
+Theorem allocR_valid :
+  forall (heapR : HeapR a) heapR' x len (valid : Valid_HeapR heapR),
+    allocR len heapR = (heapR', x) -> Valid_HeapR heapR'.
+Proof.
+  unfold allocR; simpl; intros.
+  destruct (0 <? len).
+    destruct (next heapR + len <=? heapEnd heapR) eqn:?. {
+      inversion_clear H0.
+      constructor; intros; simpl in *.
+      - destruct H0.
+        inversion_clear H0.
+          omega.
+        apply next_avail in H0; auto.
+        omega.
+      - apply Nat.leb_le in Heqb.
+        omega.
+      - apply values_allocated in H0; auto.
+        destruct H0, H0, H0.
+        exists x0, x1.
+        intros.
+        destruct H.
+        split; [|omega].
+        right; auto.
+    }
+    inversion H0; subst; clear H0.
+    assumption.
+  inversion H0; subst; clear H0.
+  assumption.
+Qed.
+
+Program Definition peekR (pos : Pos) `(!Valid_HeapR heapR) :
+  option a :=
+  match find (fun '(p, _) => pos =? p) (values heapR) with
+  | Some (_, val) => Some val
+  | None => None
+  end.
+
+Definition denote `{Monoid a} (h : HeapR a) : Rep RealHeap :=
+  fun p =>
+    match find (fun '(pos, len) => (pos <=? p) && (p <? pos + len))
+               (allocs h) with
+    | Some (pos, len) =>
+      Some (pos, len,
+            match find (fun '(pos, _) => p =? pos) (values h) with
+            | Some (_, val) => val
+            | None => mempty
+            end)
+    | None => None
+    end.
+
+Theorem refine_If_Then_Else' :
+  forall (A : Type) (c : bool) (x y r : Comp A),
+  (c = true -> refine x r) ->
+  (c = false -> refine y r) ->
+  refine (If c Then x Else y) r.
+Proof.
+  intros.
+  destruct c eqn:?; subst; simpl; intuition.
+Qed.
+
+Theorem denote_alloc heapR len (valid : Valid_HeapR heapR) :
+  refine (callMeth RealHeap allocS (denote heapR) len)
+         (match allocR len heapR with
+          | (heapR', posR) => ret (denote heapR', posR)
+          end).
+Proof.
+  simpl; unfold alloc, allocR, denote; intros.
+  apply refine_If_Then_Else'; intros.
+    refine pick val (If next heapR + len <=? heapEnd heapR
+                     Then Some (next heapR)
+                     Else None).
+      unfold Bind2.
+      simplify with monad laws; simpl.
+      destruct (next heapR + len <=? heapEnd heapR) eqn:?; simpl.
+        simplify with monad laws; simpl.
+        unfold guard.
+        pose proof H0.
+        apply Nat.ltb_lt in H1.
+        refine pick val (); auto.
+        simplify with monad laws; simpl.
+        refine pick val (next heapR).
+          simplify with monad laws; simpl.
+          refine pick val (); auto.
+          simplify with monad laws; simpl.
+          apply refine_ret_eq.
+          rewrite H0.
+          f_equal.
+          unfold Pos.
+          f_equal.
+          extensionality p.
+          simpl.
+          destruct ((next heapR <=? p) && (p <? next heapR + len)) eqn:?.
+            f_equal.
+            f_equal.
+            apply andb_prop in Heqb0.
+            destruct Heqb0.
+            apply Nat.leb_le in H2.
+            apply Nat.ltb_lt in H3.
+            destruct (find _ _) eqn:?; auto.
+            destruct p0.
+            apply find_some in Heqo.
+            destruct Heqo.
+            apply Nat.eqb_eq in H5.
+            subst.
+            pose proof (values_allocated valid _ _ H4).
+            destruct H5, H5, H5.
+            pose proof (next_avail valid _ _ H5).
+            omega.
+          reflexivity.
+        intros.
+        destruct (find _ _) eqn:?; auto.
+        destruct p0.
+        elimtype False.
+        apply find_some in Heqo.
+        destruct Heqo.
+        apply andb_prop in H4.
+        destruct H4.
+        apply Nat.leb_le in H4.
+        apply Nat.ltb_lt in H5.
+        pose proof (next_avail valid _ _ H3).
+        omega.
+      rewrite H0.
+      reflexivity.
+    destruct (next heapR + len <=? heapEnd heapR) eqn:?; simpl; auto.
+    intros.
+    destruct (find _ _) eqn:?; auto.
+    destruct p0.
+    apply find_some in Heqo.
+    destruct Heqo.
+    apply andb_prop in H3.
+    destruct H3.
+    apply Nat.leb_le in H3.
+    apply Nat.ltb_lt in H4.
+    pose proof (next_avail valid _ _ H2).
+    omega.
+  rewrite H0.
+  reflexivity.
+Qed.
+
+Theorem Heap : FullySharpened RealHeap.
+Proof.
+  start sharpening ADT.
+
+  hone representation using (fun o n => Valid_HeapR n /\ denote n = o).
+
+  {
+    simplify with monad laws.
+    refine pick val {| allocs := nil; values := nil; next := 0; heapEnd := 100 |}.
+      finish honing.
+    split; auto.
+    constructor; simpl; intros.
+    - contradiction.
+    - omega.
+    - contradiction.
+  }
+
+  {
+    destruct H1.
+    subst.
+    rewrite (denote_alloc d H1).
+    replace (let (heapR', posR) := allocR d r_n in ret (denote heapR', posR))
+       with (ret (denote (fst (allocR d r_n)), snd (allocR d r_n)))
+       by (destruct (allocR d r_n); simpl; auto).
+    simplify with monad laws; simpl.
+    refine pick val (fst (allocR d r_n)).
+      simplify with monad laws; simpl.
+      finish honing.
+    destruct (allocR d r_n) eqn:?.
+    pose proof (allocR_valid _ H1 Heqp).
+    auto.
+  }
+
+  {
+    admit.
+  }
+
+  {
+    admit.
+  }
+
+  {
+    admit.
+  }
+
+  finish_SharpeningADT_WithoutDelegation.
+Admitted.
+
+End Alloc.
